lava/coqDeps/LiquidPreludeUtil.v
@@ -124,7 +124,9 @@ Ltac solver := repeat first [
 Ltac solver_loop :=
   repeat_or_fail concat_either (quick_wff_wit) (
     concat_either (quicksolve) (
-      progress concat_either (simpl in *; timeout 1200 cleanup_after_hints) (
+      progress concat_either (
+        simpl in *; (*try timeout 2 repeat nonbranching_destruct;*)
+        timeout 1200 cleanup_after_hints) (
         lia_preprocessor
         (*concat_either (lia_preprocessor) (split_hyps)*)
       )
